First binary assembler implementation

src/asm.v
@@ -1,3 +1,127 @@
+Require Import Coq.Arith.Arith.
+Require Import Coq.omega.Omega.
+Require Import Lists.List.
+Import ListNotations.
 Require Import ast.
 
-Search dst.
+Fixpoint asm_number_rec
+         (n: N) (bit: nat) (acc: list bool): list bool :=
+  match bit with
+  | 0 => acc
+  | S b => asm_number_rec
+             n b (cons (N.testbit n (N.of_nat bit)) acc)
+  end.
+
+Definition asm_number {bits} (n: number bits): list bool :=
+  match n with
+  | num _ n _ => asm_number_rec n (pred bits) nil
+  end.
+
+Definition asm_operator_num (op: operator): N :=
+  match op with
+  | addl => 0
+  | subl => 1
+  | andl => 2
+  | xorl => 3
+  end.
+
+Fact asm_operator_4bits (op: operator):
+  (N.size_nat (asm_operator_num op)) <= 4.
+Proof. case op; size. Qed.
+
+Definition asm_operator (op: operator): list bool :=
+  (asm_number (num 4
+                   (asm_operator_num op)
+                   (asm_operator_4bits op))).
+
+Definition asm_condition_num (cond: condition): N :=
+  match cond with
+  | none => 0
+  | le => 1
+  | l => 2
+  | e => 3
+  | ne => 4
+  | ge => 5
+  | g => 6
+  end.
+
+Fact asm_condition_4bits (cond: condition):
+  N.size_nat (asm_condition_num cond) <= 4.
+Proof. case cond; size. Qed.
+
+Definition asm_condition (cond: condition): list bool :=
+  (asm_number (num 4
+                   (asm_condition_num cond)
+                   (asm_condition_4bits cond))).
+
+Definition asm_instruction (i: instruction): list bool :=
+  match i with
+  | halt =>
+    (asm_number (num 4 0 ltac:(size)))
+      ++ (asm_number (num 4 0 ltac:(size)))
+  | nop =>
+    (asm_number (num 4 1 ltac:(size)))
+      ++ (asm_number (num 4 0 ltac:(size)))
+  | rrmovl cond (reg ra) (reg rb) =>
+    (asm_number (num 4 2 ltac:(size)))
+      ++ (asm_condition cond)
+      ++ (asm_number ra)
+      ++ (asm_number rb)
+  | irmovl (imm v) (reg rb) =>
+    (asm_number (num 4 3 ltac:(size)))
+      ++ (asm_number (num 4 0 ltac:(size)))
+      ++ (asm_number (num 4 15 ltac:(size)))
+      ++ (asm_number rb)
+      ++ (asm_number v)
+  | rmmovl (reg ra) (dsp d) (reg rb) =>
+    (asm_number (num 4 4 ltac:(size)))
+      ++ (asm_number (num 4 0 ltac:(size)))
+      ++ (asm_number ra)
+      ++ (asm_number rb)
+      ++ (asm_number d)
+  | mrmovl (dsp d) (reg ra) (reg rb) =>
+    (asm_number (num 4 5 ltac:(size)))
+      ++ (asm_number (num 4 0 ltac:(size)))
+      ++ (asm_number ra)
+      ++ (asm_number rb)
+      ++ (asm_number d)
+  | OPl op (reg ra) (reg rb) =>
+    (asm_number (num 4 6 ltac:(size)))
+      ++ (asm_operator op)
+      ++ (asm_number ra)
+      ++ (asm_number rb)
+  | jump cond (dst d) =>
+    (asm_number (num 4 7 ltac:(size)))
+      ++ (asm_condition cond)
+      ++ (asm_number d)
+  | call (dst d) =>
+    (asm_number (num 4 8 ltac:(size)))
+      ++ (asm_number (num 4 0 ltac:(size)))
+      ++ (asm_number d)
+  | ret =>
+    (asm_number (num 4 9 ltac:(size)))
+      ++ (asm_number (num 4 0 ltac:(size)))
+  | pushl (reg ra) =>
+    (asm_number (num 4 10 ltac:(size)))
+      ++ (asm_number (num 4 0 ltac:(size)))
+      ++ (asm_number ra)
+      ++ (asm_number (num 4 15 ltac:(size)))
+  | popl (reg ra) =>
+    (asm_number (num 4 11 ltac:(size)))
+      ++ (asm_number (num 4 0 ltac:(size)))
+      ++ (asm_number ra)
+      ++ (asm_number (num 4 15 ltac:(size)))
+  end.
+
+Fixpoint asm_rev (ins: instructions): list bool :=
+  match ins with
+  | cons i ins => List.rev_append (asm_instruction i)
+                                  (asm_rev ins)
+  | nil => nil
+  end.
+
+Definition asm (ins: instructions): list bool :=
+  List.rev (asm_rev ins).
+
+Definition dasm (binary: list bool): option instructions :=
+  None.
